\documentclass{article}
\usepackage{amsmath,amssymb}
\newcounter{question}
\setcounter{question}{0}
\begin{document}

\newcommand\Que[1]{%
   \leavevmode\par
   \stepcounter{question}
   \noindent
   \thequestion. Q) #1\par}

\newcommand\Ans[2][]{%
    \leavevmode\par\noindent
   {A) \textbf{#1}#2\par}}

\Que{
    $ \int{7\sin^2(x)\cos^3(x)}dx $\\
    }
\Ans{
    $ I = 7\int{sin^2(x)cos^2(x)cos(x)}dx $\\

    Let $ u=\sin(x) $; $ du=\cos(x)dx $. Also $ \cos^2(x) = 1-sin^2(x) = 1-u^2 $\\

    $ \implies I = 7\int{u^2(1-u^2)}du $\\

    $ = 7\int{(u^2 - u^4)}du $\\

    $ = \frac{7u^3}{3} - \frac{7u^5}{5} + C $\\

    $ = \frac{7\sin^3(x)}{3} - \frac{7\sin^5(x)}{5} + C $\\
}
\Que{
    $ \int{19\sin^2(x)\cos^3(x)}dx $\\
    }
\Que{
    $ \int_{0}^{\pi/2}{\sin^5(x)\cos^5(x)}dx $\\
    }
\Ans{
    Let $ I = \int{\sin^5(x)\cos^5(x)}dx $\\

    Let $ u=\sin(x) $; $ du=\cos(x)dx $. Also $ \cos^2(x) = 1-sin^2(x) = 1-u^2 $\\

    $ \implies I = \int{u^5(1-u^2)^2}du $\\

    $ = \int{u^5(1-2u^2+u^4)}du $\\

    $ = \int{(u^5 - 2u^7 + u^9)}du = u^6/6 - u^8/4 + u^{10}/10 + C $\\
    
    $ = \frac{\sin^6(x)}{6} - \frac{\sin^8(x)}{4} + \frac{\sin^{10}(x)}{10} + C $\\

    $ \implies \left[I\right]_0^{\pi/2} = \frac{\sin^6(\pi/2)}{6} - \frac{\sin^8(\pi/2)}{4} + \frac{\sin^{10}(\pi/2])}{10} - 0 $\\

    $ = \frac{1}{6} - \frac{1}{4} + \frac{1}{10} = \frac{10-15+6}{60} = 1/60 $\\
}    
\Que{
    $ \int_{0}^{\pi/2}{3\cos^2(x)}dx $\\
    }
\Ans{
    Let $ I = \int{\cos^2(x)}dx $\\

    $ = \int{\frac{1+\cos(2x)}{2}}dx $\\

    $ = \int{\frac{1}{2}}dx + \int{\frac{\cos(2x)}{2}}dx $\\

    $ = \frac{x}{2} + \frac{\sin(2x)}{4} + C $\\

    $ \implies 3I_0^{\pi/2} = 3(\frac{\pi}{4} + 0 - 0) = 3\pi/4 $\\
}
\Que{
    $ \int_{0}^{\pi}{9\sin^2(x)\cos^4(x)}dx $\\
    }
\Ans{
    Let $ I = \int{\sin^2(x)\cos^4(x)}dx $\\
    
    $ = \int{\frac{1-\cos(2x)}{2}(\frac{1+\cos(2x)}{2})^2}dx $\\

    $ = \frac{1}{8}\int{(1-\cos(2x))(1+2\cos(2x)+\cos^2(2x))}dx $\\

    $ = \frac{1}{8}\int{(1+2\cos(2x)+\cos^2(2x) - \cos(2x) - 2\cos^2(2x) - \cos^3(2x))}dx $\\

    $ = \frac{1}{8}\int{(1+\cos(2x) - \cos^2(2x) - \cos^3(2x))}dx $\\
    
    $ \int{\cos(2x)}dx 
    = \frac{1}{2}\sin(2x) + C_1 
    $\\
    
    $ \int{\cos^2(2x)}dx 
    = \frac{1}{2}\int{(1+cos(4x))}dx 
    = \frac{1}{2}(x+\frac{1}{4}\sin(4x)) 
    = \frac{x}{2} + \frac{1}{8}\sin(4x) + C_2 
    $\\
    
    $ \int{\cos^3(2x)}dx 
    = \int{\cos^2(2x)\cos(2x)}dx 
    = \int{\sqrt{1-\sin^2(2x)}\cos(2x)}dx 
    = \frac{1}{2}\int{(1-u^2)^\frac{1}{2}}du $, 
    for $u=sin(2x)$ and $\frac{1}{2}du = \cos(2x)dx 
    $\\
    
    $ = -\frac{1}{2}\frac{v^{\frac{3}{2}}}{3/2} + C_3 $,
    for $ v=(1-u^2) $ and $ -\frac{1}{2}dv=udu 
    $\\

    $ = -\frac{1}{3}v^{\frac{3}{2}} + C_3 
    = -\frac{1}{3}(1-u^2)^{\frac{3}{2}} + C_3 
    = -\frac{1}{3}(1-sin^2(2x))^{\frac{3}{2}} + C_3 
    $\\

    $ \implies I 
    = \frac{1}{8}\left[
        x 
        + \frac{1}{2}\sin(2x)
        - (\frac{x}{2} + \frac{1}{8}\sin(4x))
        - (-\frac{1}{3}(1-sin^2(2x))^{\frac{3}{2}})
    \right] $\\

    $ 
    = \frac{1}{8}\left[
        \frac{x}{2}
        + \frac{1}{2}\sin(2x)
        - \frac{1}{8}\sin(4x)
        +\frac{1}{3}(1-sin^2(2x))^{\frac{3}{2}}
    \right] $\\

    $ \implies \int_{0}^{\pi}{9\sin^2(x)\cos^4(x)}dx $\\

    $
    = \frac{9}{8}\left[
        \frac{x}{2}
        + \frac{1}{2}\sin(2x)
        - \frac{1}{8}\sin(4x)
        +\frac{1}{3}(1-sin^2(2x))^{\frac{3}{2}}
    \right]_{0}^{\pi} $\\

    $
    = \frac{9}{8}\left[
        (
            \frac{\pi}{2}
            + \frac{1}{2}\sin(2\pi)
            - \frac{1}{8}\sin(4\pi)
            +\frac{1}{3}(1-sin^2(2\pi))^{\frac{3}{2}}
        )
        -
        (\frac{1}{3})
    \right] $\\

    $ = \frac{9}{8}\left[
        \frac{\pi}{2} + 0 - 0
        + \frac{1}{3}(1-0)^{\frac{3}{2}}
        - \frac{1}{3}
    \right] = \frac{9\pi}{16} $\\
}
\Que{
    $ \int{\tan^6(x)\cos^7(x)}dx $\\
    }
\Ans{
    $ = \int{{\frac{\sin^6(x)}{\cos^6(x)}}\cos^7(x)}dx $\\

    $ = \int{\sin^6(x)\cos(x)}dx $\\

    $ = \int{u^6}du $, for $u=\sin(x)$ and $du = cos(x)dx$\\

    $ = \frac{u^7}{7} + C $\\

    $ = \frac{\sin^7(x)}{7} + C $\\
}
\Que{
    $ \int{3t\sin^2(t)}dt $\\
    }
\Ans{
    $ = 3\int{uv^{\prime}}dt $, 
    for $ u=t, v^{\prime}=\sin^2(t) $, 
    therefore $ u^{\prime}=1, v=\int{\sin^2(t)}dt $\\

    $ v = \int{\frac{1-\cos(2t)}{2}}dt $\\

    $ = \int{\frac{1}{2}}dt - \int{\frac{\cos(2t)}{2}}dt $\\

    $ = \frac{t}{2} - \frac{1}{4}\sin(2t) $\\
    
    $ \int{vu^{\prime}} = \int{(\frac{t}{2} - \frac{1}{4}\sin(2t))}dt $\\

    $ = \frac{t^2}{4} + \frac{1}{8}\cos(2t) $\\

    $ \implies \int{3t\sin^2(t)}dt $\\

    $
    = 3\left[ 
        t(\frac{t}{2} - \frac{1}{4}\sin(2t))
        - (\frac{t^2}{4} + \frac{1}{8}\cos(2t))
        \right] + C $\\

    $ 
    = 3\left[ 
        \frac{t^2}{2} - \frac{t}{4}\sin(2t)
        - \frac{t^2}{4} - \frac{1}{8}\cos(2t)
        \right] + C $\\

    $ 
    = 3\left[ 
        \frac{t^2}{4}
        - \frac{t}{4}\sin(2t)
        - \frac{1}{8}\cos(2t)
        \right] + C $\\
}
\end{document}