\documentclass{article}
\usepackage{amsmath,amssymb}
\newcounter{question}
\setcounter{question}{0}
\begin{document}

\newcommand\Que[1]{%
   \leavevmode\par
   \stepcounter{question}
   \noindent
   \thequestion. Q) #1\par}

\newcommand\Ans[2][]{%
    \leavevmode\par\noindent
   {A) \textbf{#1}#2\par}}

\Que{
    Surface area of rvolution:\\

    $ x = \frac{1}{3}(y^2+2)^{3/2}, 1 \le y \le 3 $\\
    }
\Ans{
    $ 3x = (y^2+2)^{3/2} $\\

    $ (3x)^{\frac{2}{3}} = y^2+2 $\\

    $ y^2 = (3x)^{\frac{2}{3}} - 2 $\\

    $ y = ((3x)^{\frac{2}{3}} - 2)^{\frac{1}{2}}
    , \sqrt{3} \le x \le \frac{11^{3/2}}{3} $\\

    $
    y^{\prime} = 
    \frac{1}{2}
    ((3x)^{\frac{2}{3}} - 2)^{-\frac{1}{2}}
    \frac{2}{3}(3x)^{-\frac{1}{3}}
    3
    $\\

    $
    = 
    (3x)^{-\frac{1}{3}}
    ((3x)^{\frac{2}{3}} - 2)^{-\frac{1}{2}}
    $\\

    $
    [y^{\prime}]^2 = 
    \frac{
        (3x)^{-\frac{2}{3}}
    }{
        (3x)^{\frac{2}{3}} - 2
    }
    =
    \frac{
        1
    }{
        (3x)^{\frac{2}{3}} [(3x)^{\frac{2}{3}} - 2]
    }
    =
    \frac{
        1
    }{
        (3x)^{\frac{4}{3}} - 2(3x)^{\frac{2}{3}}
    }
    $\\

    $
    1 + [y^{\prime}]^2 = 
    1 + \frac{
        1
    }{
        (3x)^{\frac{4}{3}} - 2(3x)^{\frac{2}{3}}
    }
    $\\

    $
    =
    \frac{
        (3x)^{\frac{4}{3}} - 2(3x)^{\frac{2}{3}} + 1
    }{
        (3x)^{\frac{4}{3}} - 2(3x)^{\frac{2}{3}}
    }
    $\\

    $
    =
    \frac{
        [(3x)^{\frac{2}{3}} - 1]^2
    }{
        (3x)^{\frac{2}{3}} [(3x)^{\frac{2}{3}} - 2]
    }
    $\\

    $
    \sqrt{1 + [y^{\prime}]^2} = 
    \frac{
        (3x)^{\frac{2}{3}} - 1
    }{
        \sqrt{(3x)^{\frac{2}{3}} [(3x)^{\frac{2}{3}} - 2]}
    }
    $\\

    $
    = 
    \frac{
        (3x)^{\frac{2}{3}} - 1
    }{
        (3x)^{\frac{1}{3}} \sqrt{(3x)^{\frac{2}{3}} - 2}
    }
    $\\

    \begin{align*}
        S & = \int_a^b{2\pi f(x) \sqrt{1+[f^{\prime}(x)^2]}} dx\\
        & = \int_{\sqrt{3}}^{\frac{11^{3/2}}{3}}{2\pi 
            \sqrt{(3x)^{\frac{2}{3}} - 2)}
            \frac{
                (3x)^{\frac{2}{3}} - 1
            }{
                (3x)^{\frac{1}{3}} \sqrt{(3x)^{\frac{2}{3}} - 2}
            }        
            } dx\\
        & = 2\pi \int_{\sqrt{3}}^{\frac{11^{3/2}}{3}}{
            \frac{
                (3x)^{\frac{2}{3}} - 1
            }{
                (3x)^{\frac{1}{3}}
            }        
            } dx\\
        \text{Let } I & = \int{
            \frac{
                (3x)^{\frac{2}{3}} - 1
            }{
                (3x)^{\frac{1}{3}}
            }        
            } dx\\
        & = \frac{1}{3} \int{
            \frac{
                u^{\frac{2}{3}} - 1
            }{
                u^{\frac{1}{3}}
            }        
            } du
            && \text{(
                For $u=3x, dx = \frac{du}{3}$
            )}\\
        & = \frac{1}{3} \int{
            [u^{\frac{1}{3}}
            - u^{\frac{-1}{3}}]
            } du\\
        & = \frac{1}{3} [
            \frac{3}{4} u^{\frac{4}{3}}
            - \frac{3}{2} u^{\frac{2}{3}}
            ]\\
        & = \frac{u^{\frac{4}{3}}}{4} 
            - \frac{u^{\frac{2}{3}}}{2} \\
        & = \frac{(3x)^{\frac{4}{3}}}{4} 
            - \frac{(3x)^{\frac{2}{3}}}{2} \\
        S & = 2\pi \left[
            \frac{(3x)^{\frac{4}{3}}}{4} 
            - \frac{(3x)^{\frac{2}{3}}}{2}
        \right]_{\sqrt{3}}^{\frac{11^{3/2}}{3}}\\
        & = 2\pi \frac{(11^{3/2})^{\frac{4}{3}}}{4} 
            - \frac{(11^{3/2})^{\frac{2}{3}}}{2}
            - \frac{(3\sqrt{3})^{\frac{4}{3}}}{4} 
            + \frac{(3\sqrt{3})^{\frac{2}{3}}}{2}\\
        & = 2\pi \frac{121}{4} 
            - \frac{11}{2}
            - \frac{9}{4} 
            + \frac{3}{2}\\
        & = 2\pi(28 - 4)\\
        & = \boxed{48\pi}\\
    \end{align*}
}
\end{document}