\documentclass{article}
\usepackage{amsmath,amssymb}
\newcounter{question}
\setcounter{question}{0}
\begin{document}

\newcommand\Que[1]{%
   \leavevmode\par
   \stepcounter{question}
   \noindent
   \thequestion. Q) #1\par}

\newcommand\Ans[2][]{%
    \leavevmode\par\noindent
   {A) \textbf{#1}#2\par}}

\Que{ $ \int{\cos^{-1}(x)}dx $ }
\Ans
{
Let $ y = \cos^{-1}(x) $\\

$\implies x = cos(y) $\\

$\implies \frac{dx}{dy} = -\sin(y) $\\

$\implies dx = -\sin(y) dy $\\

Therefore $ \int{\cos^{-1}(x)}dx
= \int{y(-\sin(y)dy)}$\\

$= -\int{y\sin(y) dy} $\\

Let $ u=y;v^{\prime}=\sin(y) $.
Therefore $ v= -\cos(y) $\\

According to integration by parts:\\
$$\int{uv^{\prime}}=uv-\int{vu^{\prime}}$$\\

Therefore $ -\int{y\sin(y) dy} $\\

$= -(y(-\cos(y)) - \int{-\cos(y) dy}) $\\

$= y\cos(y) - \int{\cos(y) dy}$\\

$= y\cos(y) - \sin(y) + C $\\

$= \cos^{-1}(x)x - \sin(cos^{-1}(x)) + C $, 
(substituting $ y=cos^{-1}(x) $)\\

$= x\cos^{-1}(x) - \sqrt{1-x^2} + C $, 
(substituting $ \sin(cos^{-1}(x))=sqrt{1-x^2} $)\\

}
\end{document}